src/Language/PlutusIR/Semantics/SemanticEquivalence/Monotonicity.v
@@ -3,65 +3,91 @@ Require Import PlutusCert.Language.PlutusIR.Semantics.Dynamic.
 Require Import PlutusCert.Language.PlutusIR.Semantics.SemanticEquivalence.LogicalRelation.RelationalModel.
 
 Require Import Arith.
+From Coq Require Import Lia.
 
-Lemma helper : forall i k j i0,
-    i <= k ->
-    i0 < i - j ->
-    i0 < k - j.
-Proof. Admitted. 
-
-Lemma RC_monotone : forall k rho T i e e',
+Lemma RC_monotone : forall k rho T i e e' ck,
+    RD ck rho ->
     RC k T rho e e' ->  
     i <= k ->
     RC i T rho e e'.
-Proof.
-  intros k rho T i e e' RC Hle__i.
+Proof with (try solve [eauto || lia]).
+  intros k rho T i e e' ck HRD HRC Hle__i.
 
-  autorewrite with RC in RC.
   autorewrite with RC.
-
-  destruct RC as [Htyp_e [Htyp_e' RC]].
-  
-  split; auto. split; auto.
 
   intros j Hlt__j e_f Hev__e.
 
-  assert (j < k) by eauto using Nat.le_trans.
-
-  remember (RC j H e_f Hev__e) as temp.
-  clear Heqtemp. clear RC. rename temp into RC.
-
-  destruct RC as [e'_f [j' [Hev__e' RV]]].
+  apply RC_to_RV with (j := j) (e_f := e_f) in HRC as temp...
+  destruct temp as [e'_f [j' [Hev__e'_f HRV]]].
 
   exists e'_f, j'. split; auto.
-  
-  destruct T; try solve [eauto || intros; eapply RV; eauto using helper].  
-Admitted.
+
+  split. eapply RV_typable_empty_1...
+  split. eapply RV_typable_empty_2...
+
+  eapply RV_condition in HRV as HRV_cond...
+
+  destruct T.
+  - intros.
+    apply RD_sem_syn with (ck := ck) in H as temp...
+    destruct temp as [T1 [T2 [Hsyn1 Hsyn2]]].
+    remember H as HRel. clear HeqHRel.
+    apply RD_rel with (ck := ck) (T1 := T1) (T2 := T2) in HRel...
+    unfold Rel in HRel.
+    apply HRel with (j := k - j)...
+    eapply HRV_cond...
+  - destruct HRV_cond.
+    + left.
+      destruct H as [x [e_body [x' [e'_body [Heq [Heq' Hfe]]]]]].
+      eexists. eexists. eexists. eexists.
+      split... split...
+      intros. eapply Hfe...
+    + right.
+      destruct H as [f [args [f' [args' [Heq [Heq' Hfe]]]]]].
+      eexists. eexists. eexists. eexists.
+      split... split...
+      intros. apply Hfe...
+  - destruct HRV_cond as [v_0 [v'_0 [Heq [Heq' Hunwr]]]].
+    eexists. eexists.
+    split... split...
+    intros. eapply Hunwr...
+  - destruct HRV_cond as [e_body [e'_body [Heq [Heq' Hie]]]].
+    eexists. eexists.
+    split... split...
+    intros. eapply Hie...
+  - destruct HRV_cond as [sv [sv' [Heq [Heq' Hse]]]].
+    eexists. eexists.
+    split...
+  - assumption.
+  - assumption.
+Qed.
     
-Lemma RV_monotone : forall k rho T i v v',
+Lemma RV_monotone : forall k rho T i v v' ck,
+    RD ck rho ->
     RV k T rho v v' ->  
     i <= k ->
     RV i T rho v v'.
 Proof.
-  intros k rho T i v v' HRV Hlt__i.
+  intros k rho T i v v' ck HRD HRV Hlt__i.
   destruct HRV as [Hval__v [Hval__v' HRC]].
   split. auto.
   split. auto.
-  eapply RC_monotone. eauto. eauto.
+  eapply RC_monotone. eauto. eauto. eauto.
 Qed.
 
-Lemma RG_monotone : forall c rho i k env env',
+Lemma RG_monotone : forall c ck rho i k env env',
+    RD ck rho ->
     RG rho k c env env' ->  
     i <= k ->
     RG rho i c env env'.
 Proof.
   induction c.
   - intros.
-    inversion H. 
+    inversion H0. 
     subst.
     constructor.
   - intros.
-    inversion H.
+    inversion H0.
     subst.
     eapply RG_cons; eauto.
     eapply RV_monotone; eauto.
